LeanSts/BFT/Byzantine.lean
@@ -1,27 +1,30 @@
 import Mathlib.Tactic
 
-#check Finset
-
-/-- A Byzantine setting in which the Byzantine nodes are fixed ahead of time. -/
-class NonadaptiveByzantineSetting {NetAddr : Type} :=
+/-- `N` number of nodes, with at most `f` faults. -/
+class ByzantineSetting {NetAddr : Type} :=
+  /-- Set of all nodes. -/
+  nodes : Finset NetAddr
   /-- Total number of nodes. -/
   N : ℕ
   /-- Number of permitted Byzantine faults. -/
   f : ℕ
-  /-- Is this node Byzantine? -/
-  isByzantine : NetAddr → Bool
 
+  N_nodes : nodes.card = N
   N_gt_0 : 0 < N
   f_lt_N : f < N
-  -- byz_lte_f :
-  --   {n | isByzantine n = true} ≤ f
-
 
 /-- A Byzantine adversary is constrained in terms of the messages it can produce
   in a given NetworkState (which can include history information). -/
-class AdversaryConstraint {Message NetworkState : Type} :=
-  canProduceMessage : Message → NetworkState  → Prop
+class AdversaryConstraint {Packet NetworkState : Type} :=
+  canProducePacket : Packet → NetworkState  → Prop
 
-class ByzantineAdversary {NetAddr Message NetworkState : Type} :=
-  setting : @NonadaptiveByzantineSetting NetAddr
-  constraint : @AdversaryConstraint Message NetworkState
+/-- A Byzantine adversary which chooses ahead-of-time which nodes
+    are corrupted, i.e. a non-adaptive adversary. -/
+class NonadaptiveByzantineAdversary {NetAddr Packet NetworkState : Type} :=
+  setting : @ByzantineSetting NetAddr
+  constraint : @AdversaryConstraint Packet NetworkState
+
+  /-- Is this node corrupted? -/
+  isByzantine : NetAddr → Bool
+  /-- The `isByzantine` function respects the threshold `f` -/
+  byz_lte_f : (setting.nodes.filter (λ n => isByzantine n)).card ≤ setting.f
